Revert "disable tests failing because of staging issues"
This reverts commit 38284bb329f7ad46b839549e0dd5300e81313adc.

Revert "temporary fix, revert after merging"

This reverts commit f11f67fd2fc843723023179841de342762dd067f.

Revert "another bootstrapping fixe, remove after merging"

This reverts commit 98fb98924c2352aec3f9b2aa7cbfb3b6c9b872c1.

Revert "another bootstrapping issue to remove after merging"

This reverts commit 9ecfb9c11f6c660c52edf0e77404964ca83d2a9b.

Revert "hack for `try?`"

This reverts commit 973f514a76626210c0375beda1254e9a859af530.

tests/lean/run/grind_try_trace.lean
@@ -78,113 +78,111 @@ info: Try these:
 example : app [a, b] [c] = [a, b, c] := by
   try?
 
--- TODO(kmill): reenable all the following tests after stage0 update
+/--
+info: Try these:
+• (induction as, bs using app.induct) <;> grind [= app]
+• (induction as, bs using app.induct) <;> grind only [app]
+-/
+#guard_msgs (info) in
+example : app (app as bs) cs = app as (app bs cs) := by
+  try?
 
--- /--
--- info: Try these:
--- • (induction as, bs using app.induct) <;> grind [= app]
--- • (induction as, bs using app.induct) <;> grind only [app]
--- -/
--- #guard_msgs (info) in
--- example : app (app as bs) cs = app as (app bs cs) := by
---   try?
+/--
+info: Try this: (induction as, bs using app.induct) <;> grind [= app]
+-/
+#guard_msgs (info) in
+example : app (app as bs) cs = app as (app bs cs) := by
+  try? (max := 1)
 
--- /--
--- info: Try this: (induction as, bs using app.induct) <;> grind [= app]
--- -/
--- #guard_msgs (info) in
--- example : app (app as bs) cs = app as (app bs cs) := by
---   try? (max := 1)
+/--
+info: Try these:
+• · expose_names; induction as, bs_1 using app.induct <;> grind [= app]
+• · expose_names; induction as, bs_1 using app.induct <;> grind only [app]
+-/
+#guard_msgs (info) in
+example : app (app as bs) cs = app as (app bs cs) := by
+  have bs := 20 -- shadow variable in the goal
+  try?
 
--- /--
--- info: Try these:
--- • · expose_names; induction as, bs_1 using app.induct <;> grind [= app]
--- • · expose_names; induction as, bs_1 using app.induct <;> grind only [app]
--- -/
--- #guard_msgs (info) in
--- example : app (app as bs) cs = app as (app bs cs) := by
---   have bs := 20 -- shadow variable in the goal
---   try?
+/--
+info: Try these:
+• · expose_names; induction as, bs using app.induct <;> grind [= app]
+• · expose_names; induction as, bs using app.induct <;> grind only [app]
+-/
+#guard_msgs (info) in
+example : app (app as bs) cs = app as (app bs cs) := by
+  revert as bs cs
+  intro _ _ _
+  -- `as`, `bs`, and `cs` now have inaccessible names.
+  try?
 
--- /--
--- info: Try these:
--- • · expose_names; induction as, bs using app.induct <;> grind [= app]
--- • · expose_names; induction as, bs using app.induct <;> grind only [app]
--- -/
--- #guard_msgs (info) in
--- example : app (app as bs) cs = app as (app bs cs) := by
---   revert as bs cs
---   intro _ _ _
---   -- `as`, `bs`, and `cs` now have inaccessible names.
---   try?
+def concat : List α → α → List α
+  | .nil,       b => .cons b .nil
+  | .cons a as, b => .cons a (concat as b)
 
--- def concat : List α → α → List α
---   | .nil,       b => .cons b .nil
---   | .cons a as, b => .cons a (concat as b)
+attribute [simp] concat
 
--- attribute [simp] concat
+/--
+info: Try these:
+• (induction as, a using concat.induct) <;> simp_all
+• (induction as, a using concat.induct) <;> simp [*]
+-/
+#guard_msgs (info) in
+example (as : List α) (a : α) : concat as a = as ++ [a] := by
+  try? -only
 
--- /--
--- info: Try these:
--- • (induction as, a using concat.induct) <;> simp_all
--- • (induction as, a using concat.induct) <;> simp [*]
--- -/
--- #guard_msgs (info) in
--- example (as : List α) (a : α) : concat as a = as ++ [a] := by
---   try? -only
-
--- /--
--- info: Try these:
--- • (induction as, a using concat.induct) <;> simp_all
--- • ·
---   induction as, a using concat.induct
---   · simp
---   · simp [*]
--- -/
--- #guard_msgs (info) in
--- example (as : List α) (a : α) : concat as a = as ++ [a] := by
---   try? -only -merge
+/--
+info: Try these:
+• (induction as, a using concat.induct) <;> simp_all
+• ·
+  induction as, a using concat.induct
+  · simp
+  · simp [*]
+-/
+#guard_msgs (info) in
+example (as : List α) (a : α) : concat as a = as ++ [a] := by
+  try? -only -merge
 
 
--- def foo : Nat → Nat
---   | 0   => 1
---   | x+1 => foo x - 1
+def foo : Nat → Nat
+  | 0   => 1
+  | x+1 => foo x - 1
 
 
--- /--
--- info: Try this: ·
---   induction x using foo.induct
---   · grind [= foo]
---   · sorry
--- -/
--- #guard_msgs (info) in
--- example : foo x > 0 := by
---   try? +missing -only -- `try?` does not solve all subgoals.
---   sorry
+/--
+info: Try this: ·
+  induction x using foo.induct
+  · grind [= foo]
+  · sorry
+-/
+#guard_msgs (info) in
+example : foo x > 0 := by
+  try? +missing -only -- `try?` does not solve all subgoals.
+  sorry
 
--- /--
--- error: tactic 'try?' failed, consider using `grind` manually, or `try? +missing` for partial proofs containing `sorry`
--- x : Nat
--- ⊢ foo x > 0
--- -/
--- #guard_msgs (error) in
--- example : foo x > 0 := by
---   try?
+/--
+error: tactic 'try?' failed, consider using `grind` manually, or `try? +missing` for partial proofs containing `sorry`
+x : Nat
+⊢ foo x > 0
+-/
+#guard_msgs (error) in
+example : foo x > 0 := by
+  try?
 
--- @[simp] def bla : List Nat → List Nat → List Nat
---   | [],    ys => ys.reverse
---   | _::xs, ys => bla xs ys
+@[simp] def bla : List Nat → List Nat → List Nat
+  | [],    ys => ys.reverse
+  | _::xs, ys => bla xs ys
 
--- attribute [grind] List.length_reverse bla
+attribute [grind] List.length_reverse bla
 
--- /--
--- info: Try these:
--- • (induction xs, ys using bla.induct) <;> grind
--- • (induction xs, ys using bla.induct) <;> simp_all
--- • (induction xs, ys using bla.induct) <;> simp [*]
--- • (induction xs, ys using bla.induct) <;> simp only [bla, List.length_reverse, *]
--- • (induction xs, ys using bla.induct) <;> grind only [List.length_reverse, bla]
--- -/
--- #guard_msgs (info) in
--- example : (bla xs ys).length = ys.length := by
---   try?
+/--
+info: Try these:
+• (induction xs, ys using bla.induct) <;> grind
+• (induction xs, ys using bla.induct) <;> simp_all
+• (induction xs, ys using bla.induct) <;> simp [*]
+• (induction xs, ys using bla.induct) <;> simp only [bla, List.length_reverse, *]
+• (induction xs, ys using bla.induct) <;> grind only [List.length_reverse, bla]
+-/
+#guard_msgs (info) in
+example : (bla xs ys).length = ys.length := by
+  try?
