tests/lean/run/grind_constProp.lean
@@ -205,11 +205,10 @@ def evalExpr (e : Expr) : EvalM Val := do
 @[grind] theorem UnaryOp.simplify_eval (op : UnaryOp) : (op.simplify a).eval σ = (Expr.una op a).eval σ := by
   grind [UnaryOp.simplify.eq_def]
 
--- TODO(kmill): reenable test after stage0 update
--- /-- info: Try this: (induction e using Expr.simplify.induct) <;> grind -/
--- #guard_msgs (info) in
--- example (e : Expr) : e.simplify.eval σ = e.eval σ := by
---   try? (max := 1)
+/-- info: Try this: (induction e using Expr.simplify.induct) <;> grind -/
+#guard_msgs (info) in
+example (e : Expr) : e.simplify.eval σ = e.eval σ := by
+  try? (max := 1)
 
 @[simp, grind =] theorem Expr.eval_simplify (e : Expr) : e.simplify.eval σ = e.eval σ := by
   induction e, σ using Expr.simplify.induct <;> grind
@@ -305,11 +304,10 @@ theorem State.cons_le_of_eq (h₁ : σ' ≼ σ) (h₂ : σ.find? x = some v) : (
 @[grind] theorem State.join_le_left_of (h : σ₁ ≼ σ₂) (σ₃ : State) : σ₁.join σ₃ ≼ σ₂ := by
   grind
 
--- TODO(kmill): reenable test after stage0 update
--- /-- info: Try this: (induction σ₁, σ₂ using State.join.induct) <;> grind -/
--- #guard_msgs (info) in
--- example (σ₁ σ₂ : State) : σ₁.join σ₂ ≼ σ₂ := by
---   try? (max := 1)
+/-- info: Try this: (induction σ₁, σ₂ using State.join.induct) <;> grind -/
+#guard_msgs (info) in
+example (σ₁ σ₂ : State) : σ₁.join σ₂ ≼ σ₂ := by
+  try? (max := 1)
 
 @[grind] theorem State.join_le_right (σ₁ σ₂ : State) : σ₁.join σ₂ ≼ σ₂ := by
   induction σ₁, σ₂ using State.join.induct <;> grind
